pset7 did

assignments/midterm/Midterm.v
@@ -35,7 +35,15 @@ Fixpoint rightmost (tr: tree) : option nat :=
     end
   end.
   
-Fixpoint leftmost (tr : tree) : option nat := None. (* Remove [None] and fill in *)
+Fixpoint leftmost (tr : tree) : option nat := 
+  match tr with
+  | Leaf => None
+  | Node v lt _ => 
+    match lt with 
+    | Leaf => Some v
+    | _ => leftmost lt
+    end
+  end.
 (* 3 points *)
   
 Fixpoint swivel tr :=
@@ -48,7 +56,12 @@ Theorem swivel_ok : forall tr,
   leftmost tr = rightmost (swivel tr).
 (* 5 points *)
 Proof.
-Abort.
+intros.
+induction tr.
+trivial.
+simpl swivel. destruct tr1. simpl swivel. simpl rightmost. simpl leftmost. trivial.
+destruct leftmost. destruct rightmost. assumption. assumption. destruct rightmost. assumption. assumption.
+Qed.
 
 (***************************************
  ** Fibonacci Sequence
@@ -69,7 +82,7 @@ Fixpoint fib_tail_rec' n a b :=
   | S n' => fib_tail_rec' n' b (a+b)
   end.
 
-Definition fib_tail_rec n := n + 0.
+Definition fib_tail_rec n := fib_tail_rec' n 1 1.
 (* Remove [n + 0] and fill in correct definition *)
 (* 2 points *)
 
@@ -88,20 +101,52 @@ Lemma fib_succ_add: forall n,
 (* 5 points *)
 Proof.
   (* FILL IN *)
-Admitted.
+  intros.
+  assert(fib (S(S n)) = fib(n) + fib(S n)) as H.
+  - simpl. trivial.
+  - assert (S n = n + 1) as H1.
+  induct n. trivial.
+  simpl. rewrite IHn. trivial. simpl. trivial. 
+  assert(S(S n)+1=S(S(S n))) as H0.
+  simpl. rewrite <- H1. trivial.
+  assert (S (S n) = n + 2).
+  assert (n+2=n+1+1) as H2. linear_arithmetic.
+  rewrite H2. rewrite <- H1. simpl. rewrite <- H1. trivial.
+  rewrite <- H1. rewrite <- H2. rewrite H. trivial.
+Qed.
 
 Lemma fib_fib_tail_rec': forall n k,
   fib_tail_rec' n (fib k) (fib (k+1)) = fib (k+n).
 (* 5 points *)
 Proof.
   (* FILL IN *)
-Admitted.
+  induction n as [|n' IH]; intros k.
+  - simpl. rewrite Nat.add_0_r. reflexivity.
+  - simpl.
+    rewrite fib_succ_add with (n:=k).
+    assert(k+2 = k+1+1). linear_arithmetic. 
+    assert (forall l,S l= l + 1) as H1.
+    intros l. induct l. simpl. trivial. simpl. rewrite <- IHl. trivial.
+    rewrite (H1 n').
+    assert(k+(n'+1)=k+1+n'). ring.
+    rewrite H0.
+    rewrite H.
+    rewrite IH with (k := k + 1).
+    trivial.
+Qed.
 
 Theorem fib_ok : forall n, fib n = fib_tail_rec n.
 (* 5 points *)
 Proof.
   (* FILL IN *)
-Abort.
+  intros.
+  assert(fib_tail_rec' n 1 1 = fib n).
+  rewrite fib_fib_tail_rec' with (k:=0).
+  assert(0+n=n). linear_arithmetic.
+  rewrite H. trivial.
+  assert(fib_tail_rec n = fib_tail_rec' n 1 1).
+  trivial. rewrite H0. rewrite H. trivial.
+Qed.
 
 (***************************************
  ** List.rev is involutive
@@ -113,7 +158,13 @@ Import ListNotations.
 Theorem rev_involutive : forall (A:Type) (l : list A), rev (rev l) = l.
 (* 5 points *)
 Proof.
-Abort.
+induct l.
+trivial.
+simpl. 
+assert(rev (rev l ++ [a]) = [a] ++ rev(rev(l))).
+rewrite rev_app_distr. trivial.
+rewrite H. rewrite IHl. trivial.
+Qed.
 
 (***************************************
  ** Insertion sort
@@ -166,7 +217,25 @@ Check compare_eq_iff.
 (* You will need to define a function [sort] that returns a sorted version 
    of the input list based on the insertion sorting algorithm above: *)
   
-Definition sort (l : list t) : list t := l. 
+Fixpoint insert (x : t) (l : list t) : list t :=
+  match l with
+  | [] => [x]
+  | y :: ys =>
+      match compare x y with
+      | Lt => x :: y :: ys
+      | Eq => x :: y :: ys
+      | Gt => y :: insert x ys
+      end
+  end.
+
+Fixpoint sort_aux (l aux : list t) : list t :=
+  match l with
+  | [] => aux
+  | x :: xs => sort_aux xs (insert x aux)
+  end.
+
+Definition sort (l : list t) : list t := sort_aux l [].
+
 (* Remove [l] and fill in correct defintion. *)
 (* 5 points *)
 
@@ -184,15 +253,58 @@ Definition sort (l : list t) : list t := l.
 Check lt.
 Check eq.
 
-Inductive sorted : list t -> Prop := . (* FILL IN *)
+Inductive sorted : list t -> Prop := 
+    (* FILL IN *)
+  | sorted_nil : sorted []
+  | sorted_singleton : forall x, sorted [x]
+  | sorted_cons : forall x y l,
+      (lt x y \/ eq x y) ->
+      sorted (y :: l) ->
+      sorted (x :: y :: l).
 (* 5 points *)
 
 (* Prove the following theorem: the result of the [sort] function 
    returns a [sorted] list. *)
 
+Lemma insert_sorted : forall x l,
+  sorted l -> sorted (insert x l).
+Proof.
+  induction l as [|y ys IH]; intros Hsorted; simpl.
+  - apply sorted_singleton.
+  - destruct (compare x y) eqn:Hcomp.
+    + apply sorted_cons. right. apply compare_eq_iff. assumption. assumption.
+    + apply sorted_cons. left. apply compare_lt_iff. assumption. assumption.
+    + inversion Hsorted; subst.
+      * apply sorted_cons. left. apply compare_gt_iff. assumption. apply sorted_singleton.
+      * apply IH in H2 as H3. destruct (insert x (y0::l)) eqn:Heq_inserted_list.
+       apply sorted_singleton. apply sorted_cons. 
+       simpl in Heq_inserted_list. destruct (compare x y0) eqn:Hcomp'.
+       inversion Heq_inserted_list; subst.
+       left. apply compare_gt_iff in Hcomp. assumption.
+       inversion Heq_inserted_list; subst.
+       left. apply compare_gt_iff in Hcomp. assumption.
+       inversion Heq_inserted_list; subst.
+      assumption.
+      assumption.
+Qed.
+
+Lemma sort_aux_sorted : forall l acc,
+  sorted acc -> sorted (sort_aux l acc).
+Proof.
+  induction l as [| x xs IH]; intros acc Hsorted_acc; simpl.
+  - assumption.
+  - apply IH.
+    apply insert_sorted.
+    assumption.
+Qed.
+
 Theorem sort_ok : forall l, sorted (sort l).
 (* 10 points *)
 Proof.
+  intros l.
+  unfold sort.
+  apply sort_aux_sorted.
+  apply sorted_nil.
 Abort.
 
 (* Of course, one also needs to prove that the sorted list is a permutation of 
@@ -209,11 +321,42 @@ Proof.
   simplify; equality.
 Qed.
 
+Lemma insert_In : forall x l e, In e l \/ e = x -> In e (insert x l).
+Proof.
+  intros x l e H.
+  induction l as [|y ys IH]; simpl in *.
+  - destruct H as [HIn | Heq]; subst; auto.
+  - destruct H as [HIn | Heq].
+    + destruct (compare x y) eqn:Hcomp; simpl; auto. 
+      destruct HIn. 
+      * left. assumption.
+      * right. apply IH. left. assumption.
+    + subst. destruct (compare x y) eqn:Hcomp; simpl; auto.
+Qed.
+
+Lemma sort_aux_perm : forall l acc e,
+  In e l \/ In e acc -> In e (sort_aux l acc).
+Proof.
+  induction l as [|x xs IH]; intros acc e HIn; simpl.
+  - destruct HIn as [HIn_l | HIn_acc].
+    + contradiction.
+    + assumption.
+  - apply IH.
+    simpl in HIn.
+    destruct HIn as [HIn_l | HIn_acc].
+    + destruct HIn_l as [Heq_x | Hin_xs].
+      * right. subst. apply insert_In. right. reflexivity.
+      * left. assumption.
+    + right. apply insert_In. left. assumption.
+Qed.
+
 (* Now to the theorem *)
 Theorem sort_is_permutation : forall l e, In e l -> In e (sort l).
 (* 20 points *)
 Proof.
-Abort.
+  intros l e HIn.
+  unfold sort. apply sort_aux_perm. left. assumption.
+Qed.
 
 (* You may need some intermediate lemmas based on the intermediate functions 
    that you may have written down. *)
