assignments/midterm/midterm.fst
@@ -42,12 +42,12 @@ let hbeq n a b =
 
 (* 5 points *)
 val hbeq_reflexive : n:nat -> v:t n -> Lemma (ensures (hbeq n v v))
-let hbeq_reflexive n v = admit ()
+let hbeq_reflexive n v = ()
 
 (* 10 points *)
 val hbeq_transitive : n:nat -> v1:t n -> v2:t n{hbeq n v1 v2} -> v3:t n{hbeq n v2 v3}
                     -> Lemma (ensures (hbeq n v1 v3))
-let hbeq_transitive n v1 v2 v3 = admit ()
+let hbeq_transitive n v1 v2 v3 = ()
 
 val concurrent : n:nat -> v1:t n -> v2:t n -> bool
 let concurrent n v1 v2 = compare v1 v2 = Concurrent
@@ -55,4 +55,4 @@ let concurrent n v1 v2 = compare v1 v2 = Concurrent
 (* 15 points *)
 val concurrent_commutative : n:nat -> v1:t n -> v2:t n{concurrent n v1 v2}
                            -> Lemma (ensures (concurrent n v2 v1))
-let concurrent_commutative n v1 v2 = admit ()
+let concurrent_commutative n v1 v2 = ()
